Prove coerce typing in pDOT

translation/TestEquality.v
@@ -10,23 +10,24 @@ Definition p_coerce_typ : typ :=
 Parameter refl : trm_label. (* TODO automatically generating constructor ids *)
 
 Definition env_typ : typ :=
-  μ
-    { GN Eq ==
-      μ
-        {Ai 1 >: ⊥ <: ⊤} ∧ {Ai 2 >: ⊥ <: ⊤}
-      ∧ {pmatch ⦂ ∀ ({GenT >: ⊥ <: ⊤})
-                      ∀ ( ∀ (ssuper ↓ GC Eq 0 ∧ {{super}} ) (this ↓ GenT))
-                        (super ↓ GenT)
+  μ (
+      { GN Eq ==
+        μ
+          {Ai 1 >: ⊥ <: ⊤} ∧ {Ai 2 >: ⊥ <: ⊤}
+        ∧ {pmatch ⦂ ∀ ({GenT >: ⊥ <: ⊤})
+                        ∀ ( ∀ (ssuper ↓ GC Eq 0 ∧ {{super}} ) (super ↓ GenT))
+                          (super ↓ GenT)
+          }
+      }
+      ∧ { GC Eq 0 ==
+          μ
+            super ↓ GN Eq
+          ∧ {Bi 1 >: ⊥ <: ⊤}
+          ∧ {Ai 1 == this ↓ Bi 1} ∧ {Ai 2 == this ↓ Bi 1}
+          ∧ {data ⦂ ssuper ↓ Unit}
         }
-    }
-  ∧ { GC Eq 0 ==
-      μ
-        this ↓ GN Eq
-      ∧ {Bi 1 >: ⊥ <: ⊤}
-      ∧ {Ai 1 == this ↓ Bi 1} ∧ {Ai 2 == this ↓ Bi 1}
-      ∧ {data ⦂ super ↓ Unit}
-    }
-  ∧ { refl ⦂ ( ∀ ({Bi 1 >: ⊥ <: ⊤}) (super ↓ GC Eq 0) ∧ {Bi 1 == this ↓ Bi 1}) }
+      ∧ { refl ⦂ ( ∀ ({Bi 1 >: ⊥ <: ⊤}) (super ↓ GC Eq 0) ∧ {Bi 1 == this ↓ Bi 1}) }
+    )
 .
 
 Definition env_trm : trm.
@@ -73,11 +74,43 @@ Definition p_coerce_trm : trm :=
     )
     .
 
+Ltac cleanup :=
+  repeat
+    match goal with
+    | [ H: ?x <> ?y |- _ ] => clear H
+    | [ H: ?x = ?y |- _ ] =>
+      match x with
+      | y => clear H
+      end
+    end.
+
+Ltac var_subtyp :=
+  match goal with
+  | [ |- ?G ⊢ tvar ?x : ?T ] =>
+    match goal with
+    | [ |- context [x ~ ?BT] ] =>
+      apply ty_sub with BT
+    end
+  end.
+
+Ltac solve_bind :=
+  repeat progress (
+           lazymatch goal with
+           | |- binds ?Var ?What (?Left & ?Right) =>
+    match goal with
+    | |- binds Var What (Left & Var ~ ?Sth) =>
+      apply* binds_concat_right; apply* binds_single_eq
+    | _ => apply* binds_concat_left
+    end
+           end).
+
 Lemma p_coerce_types :
-    empty & lib ~ libType & env ~ env_typ ⊢
-                                p_coerce_trm : p_coerce_typ.
-  lets lib: lib.
-  lets env: env.
+  empty & lib ~ libType
+  & env ~ (open_typ_p (pvar lib) env_typ)
+        ⊢
+        p_coerce_trm : p_coerce_typ.
+  remember lib as lib.
+  remember env as env.
   intros.
   cbv.
   crush.
@@ -93,16 +126,136 @@ Lemma p_coerce_types :
       assert (HR: open_typ_p (pvar μt) {GenT == pvar B ↓ GenT} = {GenT == pvar B ↓ GenT}) by crush.
       rewrite <- HR at 2.
       apply ty_rec_elim. crush.
-  - apply_fresh ty_let as c0case; crush.
-    + admit.
+  - cleanup.
+    apply_fresh ty_let as c0case; crush.
+    + instantiate (1:= ∀ (pvar env ↓ GC Eq 0 ∧ {{pvar eq}} ) (pvar TL ↓ GenT) ).
+      repeat rewrite <- Heqenv.
+      apply_fresh ty_all_intro as eq_ev; crush.
+      apply ty_sub with (pvar A ↓ GenT).
+      * apply ty_var. crush.
+      * apply subtyp_trans with (pvar B ↓ GenT).
+        2: {
+          eapply subtyp_sel2.
+          crush.
+        }
+        apply subtyp_trans with (pvar eq_ev ↓ Bi 1).
+        -- apply subtyp_trans with (pvar eq ↓ Ai 2).
+           ++ eapply subtyp_sel2.
+              var_subtyp; crush.
+           ++ apply subtyp_trans with (pvar eq_ev ↓ Ai 2).
+              ** eapply subtyp_sngl_qp with (p := pvar eq_ev) (q := pvar eq);
+                   try solve [var_subtyp; crush].
+                 assert (HR: pvar eq_ev = (pvar eq_ev) •• []) by crush.
+                 rewrite HR at 2.
+                 assert (HR2: pvar eq = (pvar eq) •• []) by crush.
+                 rewrite HR2 at 2.
+                 apply rpath.
+              ** eapply subtyp_sel1.
+                 apply ty_sub with (((((pvar env ↓ GN Eq) ∧ {Bi 1 >: ⊥ <: ⊤}) ∧ {Ai 1 == pvar eq_ev ↓ Bi 1}) ∧ {Ai 2 == pvar eq_ev ↓ Bi 1}) ∧ {data ⦂ pvar lib ↓ Unit}).
+                 ---
+                   assert (HR:
+                             ((((pvar env ↓ GN Eq) ∧ {Bi 1 >: ⊥ <: ⊤}) ∧ {Ai 1 == pvar eq_ev ↓ Bi 1})
+                              ∧ {Ai 2 == pvar eq_ev ↓ Bi 1}) ∧ {data ⦂ pvar lib ↓ Unit}
+                                      =
+                                      open_typ_p (pvar eq_ev) (((((pvar env ↓ GN Eq) ∧ {Bi 1 >: ⊥ <: ⊤}) ∧ {Ai 1 == this ↓ Bi 1}) ∧ {Ai 2 == this ↓ Bi 1}) ∧ {data ⦂ pvar lib ↓ Unit})) by crush.
+                   rewrite HR.
+                   apply ty_rec_elim.
+                   apply ty_sub with (pvar env ↓ GC Eq 0).
+                   +++ var_subtyp; crush.
+                   +++ eapply subtyp_sel1.
+                       match goal with
+                       | [ |- context [ env ~ μ ?T ] ] =>
+                         apply ty_sub with (open_typ_p (pvar env) T)
+                       end.
+                       *** apply ty_rec_elim. apply ty_var.
+                           solve_bind.
+                       *** crush.
+                           eapply subtyp_trans; try apply subtyp_and11.
+                           apply subtyp_and12.
+                 --- eapply subtyp_trans; try apply subtyp_and11.
+                     apply subtyp_and12.
+        -- apply subtyp_trans with (pvar eq ↓ Ai 1).
+           ++ apply subtyp_trans with (pvar eq_ev ↓ Ai 1).
+              ** eapply subtyp_sel2.
+                 apply ty_sub with (((((pvar env ↓ GN Eq) ∧ {Bi 1 >: ⊥ <: ⊤}) ∧ {Ai 1 == pvar eq_ev ↓ Bi 1}) ∧ {Ai 2 == pvar eq_ev ↓ Bi 1}) ∧ {data ⦂ pvar lib ↓ Unit}).
+                 ---
+                   assert (HR:
+                             ((((pvar env ↓ GN Eq) ∧ {Bi 1 >: ⊥ <: ⊤}) ∧ {Ai 1 == pvar eq_ev ↓ Bi 1})
+                              ∧ {Ai 2 == pvar eq_ev ↓ Bi 1}) ∧ {data ⦂ pvar lib ↓ Unit}
+                                      =
+                                      open_typ_p (pvar eq_ev) (((((pvar env ↓ GN Eq) ∧ {Bi 1 >: ⊥ <: ⊤}) ∧ {Ai 1 == this ↓ Bi 1}) ∧ {Ai 2 == this ↓ Bi 1}) ∧ {data ⦂ pvar lib ↓ Unit})) by crush.
+                   rewrite HR.
+                   apply ty_rec_elim.
+                   apply ty_sub with (pvar env ↓ GC Eq 0).
+                   +++ var_subtyp; crush.
+                   +++ eapply subtyp_sel1.
+                       match goal with
+                       | [ |- context [ env ~ μ ?T ] ] =>
+                         apply ty_sub with (open_typ_p (pvar env) T)
+                       end.
+                       *** apply ty_rec_elim. apply ty_var.
+                           solve_bind.
+                       *** crush.
+                           eapply subtyp_trans; try apply subtyp_and11.
+                           apply subtyp_and12.
+                 --- eapply subtyp_trans; try apply subtyp_and11.
+                     eapply subtyp_trans; try apply subtyp_and11.
+                     apply subtyp_and12.
+              ** eapply subtyp_sngl_pq with (p := pvar eq_ev) (q := pvar eq);
+                   try solve [var_subtyp; crush].
+                 assert (HR: pvar eq_ev = (pvar eq_ev) •• []) by crush.
+                 rewrite HR at 2.
+                 assert (HR2: pvar eq = (pvar eq) •• []) by crush.
+                 rewrite HR2 at 2.
+                 apply rpath.
+           ++ eapply subtyp_sel1.
+              var_subtyp; crush.
+              eapply subtyp_trans; try apply subtyp_and11.
+              apply subtyp_and12.
     + apply_fresh ty_let as app_tmp1; crush.
-      * admit.
+      * instantiate (1:= open_typ_p (pvar TL) (∀ ( ∀ (pvar env ↓ GC Eq 0 ∧ {{pvar eq}} ) (super ↓ GenT) ) (super ↓ GenT))).
+        eapply ty_all_elim.
+        2: {
+          apply ty_var. crush.
+        }
+        assert (HR: p_sel (avar_f eq) [pmatch] = (pvar eq) • pmatch) by crush.
+        rewrite HR.
+
+        match goal with
+        | [ |- ?G ⊢ ?t : ∀ (?T) ?U ] =>
+          apply ty_sub with (∀ ({GenT >: ⊥ <: ⊤}) U)
+        end.
+        --
+          apply ty_new_elim.
+          apply ty_sub with (open_typ_p (pvar eq) (({Ai 1 >: ⊥ <: ⊤} ∧ {Ai 2 >: ⊥ <: ⊤})
+        ∧ {pmatch
+          ⦂ ∀ ({GenT >: ⊥ <: ⊤}) (∀ (∀ ((pvar env ↓ GC Eq 0) ∧ {{super}})
+                                       (super ↓ GenT)) (super ↓ GenT) ) })).
+          ++ apply ty_rec_elim.
+             apply ty_sub with (pvar env ↓ GN Eq).
+             ** var_subtyp; crush.
+                repeat rewrite <- Heqenv.
+                eapply subtyp_trans; apply subtyp_and11.
+             ** eapply subtyp_sel1.
+                match goal with
+                | [ |- context [ env ~ μ ?T ] ] =>
+                  apply ty_sub with (open_typ_p (pvar env) T)
+                end.
+                *** apply ty_rec_elim. apply ty_var.
+                    solve_bind.
+                *** crush.
+                    eapply subtyp_trans; try apply subtyp_and11.
+          ++ crush.
+        -- apply_fresh subtyp_all as TLL; crush.
       * apply_fresh ty_let as res_tmp.
-        -- admit.
-        -- admit.
-        (* instantiate (1:= ∀ ( ∀ (pvar env ↓ GC Eq 0 ∧ {{pvar eq}} ) (pvar TL ↓ GenT) )
-                        (pvar TL ↓ GenT)). *)
-Admitted.
+        -- crush.
+           instantiate (1 := open_typ_p (pvar c0case) (pvar TL ↓ GenT)).
+           eapply ty_all_elim; crush.
+        -- crush.
+           apply ty_sub with (pvar TL ↓ GenT); crush.
+           eapply subtyp_sel1.
+           crush.
+Qed.
 
 Definition p_transitivity_typ := translateTyp0 transitivity_typ.
 
